\begin{align}
  y_0 & = \mu_0+\mu_1 x_0+\mu_2 x_0^{2}+\mu_3 x_0^{3}  \\
   y_1 & = \mu_0+\mu_1 x_1+\mu_2 x_1^{2}+\mu_3 x_1^{3}  \\
   d_0 & =  \mu_1+2 \mu_2 x_0+3 \mu_3 x_0^{2}  \\
   d_1 & = \mu_1+2 \mu_2 x_1+3 \mu_3 x_1^{2}  
\end{align}

 
\begin{align}
  \mu_0 & =  \left(  -  \left( d_0 x_1+d_1 x_0 \right)   \left( x_0 - x_1 \right)  x_0 x_1+x_0^{3} y_1 - 3  x_0^{2} x_1 y_1+3 x_0 x_1^{2} y_0 - x_1^{3} y_0 \right)  /  \left( x_0 - x_1 \right) ^{3}  \\
   \mu_1  & =  \left(  \left(  \left( x_0+2 x_1 \right)   \left( x_0 - x_1 \right)  d_1 - 6  \left( y_0 - y_1  \right)  x_1 \right)  x_0+ \left( 2 x_0+x_1 \right)   \left( x_0 - x_1 \right)  d_0 x_1  \right)  /  \left( x_0 - x_1 \right) ^{3}  \\
   \mu_2 & =  \left(  -  \left(  \left( x_0+2 x_1 \right)    \left( x_0 - x_1 \right)  d_0 - 3  \left( x_0+x_1 \right)   \left( y_0 - y_1 \right)  \right)  -   \left( 2 x_0+x_1 \right)   \left( x_0 - x_1 \right)  d_1 \right)  /  \left( x_0 - x_1 \right) ^{3}   \\
   \mu_3 & =  \left(  \left( d_0+d_1 \right)   \left( x_0 - x_1 \right)  - 2  \left( y_0 - y_1 \right)   \right)  /  \left( x_0 - x_1 \right) ^{3}  
\end{align}
