\begin{align}
  y_0 & = a_0+a_1 x_0+a_2 x_0^{2}+a_3 x_0^{3}  \\
   y_1 & = a_0+a_1 x_1+a_2 x_1^{2}+a_3 x_1^{3}  \\
   d_0 & =  a_1+2 a_2 x_0+3 a_3 x_0^{2}  \\
   d_1 & = a_1+2 a_2 x_1+3 a_3 x_1^{2}  
\end{align}

 
\begin{align}
   a_0 & = \left(x_0^{3} y_1 - 3 x_0^{2} x_1 y_1+3 x_0 x_1^{2} y_0 - x_1^{3} y_0 - \left(x_0 - x_1 \right) d_1 x_0^{2} x_1 - \left(x_0 - x_1\right) d_0 x_0 x_1^{2}\right)/\left(x_0 - x_1 \right)^{3}  \\
   a_1 & = \left(\left(\left(x_0+2 x_1\right) \left(x_0 - x_1\right) d_1 -  6 \left(y_0 - y_1\right) x_1\right) x_0+\left(2 x_0+x_1\right) \left(x_0 - x_1 \right) d_0 x_1\right)/\left(x_0 - x_1\right)^{3}  \\
   a_2 & = \left( - \left(\left(2 x_0 +x_1\right) \left(x_0 - x_1\right) d_1 - 3 \left(x_0+x_1\right) \left(y_0 - y_1\right) +\left(x_0+2 x_1\right) \left(x_0 - x_1\right) d_0\right)\right)/\left(x_0 - x_1 \right)^{3}  \\
   a_3 & = \left(\left(x_0 - x_1\right) d_1 - 2 \left(y_0 - y_1\right)+\left( x_0 - x_1\right) d_0\right)/\left(x_0 - x_1\right)^{3}   
\end{align}
