\begin{align}
  y_0 & = a_0+a_1 x_0+a_2 x_0^{2}  \\
   y_1 & = a_0+a_1 x_1+a_2 x_1^{2}  \\
   d_2 & = a_1+2 a_2 x_2  
\end{align}

 
\begin{align}
   a_0 & = \frac
{\left(x_0 - 2 x_2\right) x_0 y_1 - \left(x_1 - 2 x_2\right) x_1 y_0 - \left(x_0 -  x_1\right) d_2 x_0 x_1}
{\left(x_0+x_1 - 2 x_2\right) \left(x_0 - x_1 \right)} \\
   a_1 & = \frac
{\left(x_0+x_1\right) \left(x_0 - x_1\right) d_2 - 2  \left(y_0 - y_1\right) x_2}
{\left(x_0+x_1 - 2 x_2\right) \left(x_0 - x_1 \right)} \\
   a_2 & = \frac
{ - \left(\left(x_0 - x_1\right) d_2 - \left(y_0 - y_1 \right)\right)}
{\left(x_0+x_1 - 2 x_2\right) \left(x_0 - x_1\right) } 
\end{align}
