\begin{align}
  y_0 & = a_0+a_1 x_0+a_2 x_0^{2}  \\
   y_1 & = a_0+a_1 x_0+a_2 x_1^{2}  \\
   d_1 & = a_1+2 a_2 x_1  
\end{align}

 
\begin{align}
   a_0 & = \frac
{x_0^{2} y_1 - x_1^{2} y_0+2 \left(y_0 - y_1\right) x_0 x_1 - \left(x_0+x_1 \right) \left(x_0 - x_1\right) d_1 x_0}
{\left(x_0+x_1\right) \left( x_0 - x_1\right)} \\
   a_1 & = \frac
{\left(x_0+x_1\right) \left(x_0 - x_1\right) d_1 -  2 \left(y_0 - y_1\right) x_1}
{\left(x_0+x_1\right) \left(x_0 - x_1 \right)} \\
   a_2 & = \frac
{y_0 - y_1}
{\left(x_0+x_1\right) \left(x_0  - x_1\right)} 
\end{align}
