\begin{align}
  0 & = a^{2}+2 a x_1 - 4 a x_3 - b^{2} - 2 x_1 x_3+3 x_3^{2}  \\
   0 & = a^{2}+2 a x_1 - 4 a x_2 - b^{ 2} - 2 x_1 x_2+3 x_2^{2}  
\end{align}

\begin{align}
   a & =  \left(  - 2 x_1+3 x_2+3 x_3 \right)  / 4  \\
   b & =  \left( \sqrt { - 4 x_1^{2}+4 x_1 x_2+4 x_1  x_3+3 x_2^{2} - 10 x_2 x_3+3 x_3^{2}} \sqrt {3} \right)  / 4   \\
    a & =  \left(  - 2 x_1+3 x_2+ 3 x_3 \right)  / 4  \\
   b & =  \left(  - \sqrt { - 4 x_1^{2}+4 x_1 x_2+4 x_1 x_3+3 x_2^{2} - 10 x_2  x_3+3 x_3^{2}} \sqrt {3} \right)  / 4   
\end{align}
