\begin{align}
  y_0 & = \mu_0+\mu_1 x_0+\mu_2 x_0^{2}  \\
   y_1 & = \mu_0+\mu_1 x_0+\mu_2 x_1^{2}  \\
   d_1 & = \mu_1+2 \mu_2 x_1  
\end{align}

 
\begin{align}
  \mu_0 & = \frac
{x_0^{2} y_1 - x_1^{2} y_0+2  \left( y_0 - y_1 \right)  x_0 x_1 -  \left( x_0+x_1  \right)   \left( x_0 - x_1 \right)  d_1 x_0}
{ \left( x_0+x_1 \right)   \left(  x_0 - x_1 \right) } \\
   \mu_1 & = \frac
{ \left( x_0+x_1 \right)   \left( x_0 - x_1 \right)  d_1 -  2  \left( y_0 - y_1 \right)  x_1}
{ \left( x_0+x_1 \right)   \left( x_0 - x_1  \right) } \\
   \mu_2 & = \frac
{y_0 - y_1}
{ \left( x_0+x_1 \right)   \left( x_0  - x_1 \right) } 
\end{align}
